Made chapter03/exercise02 camera-ready

chapter03/exercises/exercise02.dfy
@@ -1,13 +1,5 @@
 // Dining Philosophers
 
-//#instructor 
-//#instructor 
-//#instructor Relative to the coke machine, the students need to
-//#instructor write their own datatype for philosophers and pair
-//#instructor (or equivalent concepts)
-//#instructor Introduces the constants idiom.
-//#instructor 
-
 // Define the state machine for the Dining Philosophers.
 // There are N philosophers sitting around a round table. 
 // Between every pair of philosophers lies a chopstick.
@@ -18,111 +10,42 @@
 
 datatype Constants = Constants(tableSize:nat)
 
-//#elide datatype Pair = Pair(left:bool, right:bool)
-datatype Variables = Variables(
-//#elide     philosophers:seq<Pair>
-)
+//Use this datatype to define all the relevant state
+datatype Variables = Variables()
 
+// An initial predicate to define well-formed constants. 
+// Feel free to add more if you need them
 predicate WellFormedConstants(c:Constants) {
     && 0 < c.tableSize 
 }
 
+
+// An initial predicate to define well-formed state. 
+// Feel free to add to this predicate, if necessary
 predicate WellFormed(c:Constants, v:Variables) {
     && WellFormedConstants(c)
-//#elide    && |v.philosophers| == c.tableSize
 }
 
 predicate Init(c:Constants, v:Variables) {
-//#elide    && WellFormed(c, v)
-//#elide    && (forall pi | 0 <= pi < |v.philosophers| :: v.philosophers[pi] == Pair(false, false))
+    true // Replace me
 }
 
+// Philosopher with index pi acquires left chopstick
 predicate AcquireLeft(c:Constants, v:Variables, v':Variables, pi:nat) {
-//#elide    && WellFormed(c, v)
-//#elide    && pi < c.tableSize
-//#elide    && !(v.philosophers[pi].left) // prevents this action from being a no-op
-//#elide    && !(v.philosophers[PhilosopherToTheLeftOf(c,pi)].right) // comment this line to create bug
-//#elide    && v' == v.(philosophers := v.philosophers[pi := Pair(true, v.philosophers[pi].right)])
+    true // Replace me
 }
 
+// Philosopher with index pi acquires right chopstick
 predicate AcquireRight(c:Constants, v:Variables, v':Variables, pi:nat) {
-//#elide    && WellFormed(c, v)
-//#elide    && pi < c.tableSize
-//#elide    && !(v.philosophers[pi].right) // prevents this action from being a no-op
-//#elide    && !(v.philosophers[PhilosopherToTheRightOf(c,pi)].left) // comment this line to create bug
-//#elide    && v' == v.(philosophers := v.philosophers[pi := Pair(v.philosophers[pi].left, true)])
+    true // Replace me
 }
 
+// Philosopher with index pi releases both chopsticks
 predicate ReleaseBoth(c:Constants, v:Variables, v':Variables, pi:nat) {
-//#elide    && WellFormed(c, v)
-//#elide    && pi < c.tableSize
-//#elide    && (v.philosophers[pi].left)
-//#elide    && (v.philosophers[pi].right)
-//#elide    && v' == v.(philosophers := v.philosophers[pi := Pair(false, false)])
+    true // Replace me
 }
  
 predicate Next(c:Constants, v:Variables, v':Variables) {
-//#elide    exists pi:nat :: 
-//#elide    (|| AcquireLeft(c, v, v', pi)
-//#elide     || AcquireRight(c, v, v', pi)
-//#elide     || ReleaseBoth(c, v, v', pi))
+    true // Replace me
 }
 
-//#elidefunction PhilosopherToTheLeftOf(c:Constants, i:nat) : nat 
-//#elide    requires WellFormedConstants(c)
-//#elide{
-//#elide    (i+1) % c.tableSize
-//#elide}
-//#elide
-//#elidefunction PhilosopherToTheRightOf(c:Constants, i:nat) : nat 
-//#elide    requires WellFormedConstants(c)
-//#elide{
-//#elide    (i-1) % c.tableSize
-//#elide}
-//#elide
-//#elide// here is the safety property
-//#elidepredicate ForkConsistency(c:Constants, v:Variables) 
-//#elide{
-//#elide    && WellFormed(c, v)
-//#elide    && (forall i | 0 <= i < c.tableSize :: !(
-//#elide        && v.philosophers[i].right 
-//#elide        && v.philosophers[PhilosopherToTheRightOf(c,i)].left
-//#elide        ))
-//#elide}
-//#elide
-//#elide// here is a proof of the safety property. This lemma should verify
-//#elide// without adding a body 
-//#elidelemma ForkConsistencyLemma() 
-//#elide    ensures forall c, v | Init(c,v) :: ForkConsistency(c, v)
-//#elide    ensures forall c, v, v' | ForkConsistency(c, v) && Next(c, v, v') :: ForkConsistency(c, v')
-//#elide{
-//#elide}
-//#elide
-//#elide// this predicate and the following lemma are a way to prevent trivial
-//#elide// specifications of the problem that would prevent a philosopher from
-//#elide// having both forks
-//#elidepredicate PhilosopherHasBothForks(c:Constants, v:Variables, pi:nat)
-//#elide    requires pi < c.tableSize
-//#elide    requires WellFormed(c, v)
-//#elide{
-//#elide    && v.philosophers[pi].left
-//#elide    && v.philosophers[pi].right
-//#elide}
-//#elide
-//#elidelemma PseudoLiveness(c:Constants, pi:nat) returns (b:seq<Variables>)
-//#elide    requires c.tableSize == 3
-//#elide    requires pi == 1
-//#elide    ensures 0 < |b| 
-//#elide    ensures Init(c, b[0])
-//#elide    ensures forall i | 0 <= i < |b|-1 :: Next(c, b[i], b[i+1])
-//#elide    ensures WellFormed(c, b[|b|-1])
-//#elide    ensures PhilosopherHasBothForks(c, b[|b|-1], pi)
-//#elide{
-//#elide    var s0 := Variables([Pair(false,false), Pair(false, false), Pair(false, false)]);
-//#elide    var s1 := Variables([Pair(false,false), Pair(true, false), Pair(false, false)]);
-//#elide    var s2 := Variables([Pair(false,false), Pair(true, true), Pair(false, false)]);
-//#elide    assert AcquireLeft(c, s0, s1, 1); // witness
-//#elide    assert AcquireRight(c, s1, s2, 1); // witness
-//#elide    b := [s0, s1, s2];
-//#elide}
-//#elide
