chapter03/solutions/exercise02_solution.dfy
@@ -1,0 +1,126 @@
+// Dining Philosophers
+
+//#instructor 
+//#instructor 
+//#instructor Relative to the coke machine, the students need to
+//#instructor write their own datatype for philosophers and pair
+//#instructor (or equivalent concepts)
+//#instructor Introduces the constants idiom.
+//#instructor 
+
+// Define the state machine for the Dining Philosophers.
+// There are N philosophers sitting around a round table. 
+// Between every pair of philosophers lies a chopstick.
+// Every philosopher has three possible actions:
+//  * Acquire the chopstick to their left.
+//  * Acquire the chopstick to their right.
+//  * Release both chopsticks (in a single step). 
+
+datatype Constants = Constants(tableSize:nat)
+
+datatype Pair = Pair(left:bool, right:bool)
+datatype Variables = Variables(philosophers:seq<Pair>)
+
+predicate WellFormedConstants(c:Constants) {
+    && 0 < c.tableSize 
+}
+
+predicate WellFormed(c:Constants, v:Variables) {
+    && WellFormedConstants(c)
+    && |v.philosophers| == c.tableSize
+}
+
+predicate Init(c:Constants, v:Variables) {
+    && WellFormed(c, v)
+    && (forall pi | 0 <= pi < |v.philosophers| :: v.philosophers[pi] == Pair(false, false))
+}
+
+predicate AcquireLeft(c:Constants, v:Variables, v':Variables, pi:nat) {
+    && WellFormed(c, v)
+    && pi < c.tableSize
+    && !(v.philosophers[pi].left) // prevents this action from being a no-op
+    && !(v.philosophers[PhilosopherToTheLeftOf(c,pi)].right) // comment this line to create bug
+    && v' == v.(philosophers := v.philosophers[pi := Pair(true, v.philosophers[pi].right)])
+}
+
+predicate AcquireRight(c:Constants, v:Variables, v':Variables, pi:nat) {
+    && WellFormed(c, v)
+    && pi < c.tableSize
+    && !(v.philosophers[pi].right) // prevents this action from being a no-op
+    && !(v.philosophers[PhilosopherToTheRightOf(c,pi)].left) // comment this line to create bug
+    && v' == v.(philosophers := v.philosophers[pi := Pair(v.philosophers[pi].left, true)])
+}
+
+predicate ReleaseBoth(c:Constants, v:Variables, v':Variables, pi:nat) {
+    && WellFormed(c, v)
+    && pi < c.tableSize
+    && (v.philosophers[pi].left)
+    && (v.philosophers[pi].right)
+    && v' == v.(philosophers := v.philosophers[pi := Pair(false, false)])
+}
+ 
+predicate Next(c:Constants, v:Variables, v':Variables) {
+    exists pi:nat :: 
+    (|| AcquireLeft(c, v, v', pi)
+     || AcquireRight(c, v, v', pi)
+     || ReleaseBoth(c, v, v', pi))
+}
+
+function PhilosopherToTheLeftOf(c:Constants, i:nat) : nat 
+    requires WellFormedConstants(c)
+{
+    (i+1) % c.tableSize
+}
+
+function PhilosopherToTheRightOf(c:Constants, i:nat) : nat 
+    requires WellFormedConstants(c)
+{
+    (i-1) % c.tableSize
+}
+
+// here is the safety property
+predicate ForkConsistency(c:Constants, v:Variables) 
+{
+    && WellFormed(c, v)
+    && (forall i | 0 <= i < c.tableSize :: !(
+        && v.philosophers[i].right 
+        && v.philosophers[PhilosopherToTheRightOf(c,i)].left
+        ))
+}
+
+// here is a proof of the safety property. This lemma should verify
+// without adding a body 
+lemma ForkConsistencyLemma() 
+    ensures forall c, v | Init(c,v) :: ForkConsistency(c, v)
+    ensures forall c, v, v' | ForkConsistency(c, v) && Next(c, v, v') :: ForkConsistency(c, v')
+{
+}
+
+// this predicate and the following lemma are a way to prevent trivial
+// specifications of the problem that would prevent a philosopher from
+// having both forks
+predicate PhilosopherHasBothForks(c:Constants, v:Variables, pi:nat)
+    requires pi < c.tableSize
+    requires WellFormed(c, v)
+{
+    && v.philosophers[pi].left
+    && v.philosophers[pi].right
+}
+
+lemma PseudoLiveness(c:Constants, pi:nat) returns (b:seq<Variables>)
+    requires c.tableSize == 3
+    requires pi == 1
+    ensures 0 < |b| 
+    ensures Init(c, b[0])
+    ensures forall i | 0 <= i < |b|-1 :: Next(c, b[i], b[i+1])
+    ensures WellFormed(c, b[|b|-1])
+    ensures PhilosopherHasBothForks(c, b[|b|-1], pi)
+{
+    var s0 := Variables([Pair(false,false), Pair(false, false), Pair(false, false)]);
+    var s1 := Variables([Pair(false,false), Pair(true, false), Pair(false, false)]);
+    var s2 := Variables([Pair(false,false), Pair(true, true), Pair(false, false)]);
+    assert AcquireLeft(c, s0, s1, 1); // witness
+    assert AcquireRight(c, s1, s2, 1); // witness
+    b := [s0, s1, s2];
+}
+
